---
title: "Trigonometry (2/5): Formulas"
subtitle: Introduction to Engineering Mathematics
author: Prof. Joris Vankerschaver
format:
  beamer:
    theme: Pittsburgh
    colortheme: default
    fonttheme: default
    include-in-header:
      - file: header.tex

classoption: t
---

## Overview

\tableofcontents

## Notes for this chapter

- You should learn all of these formulas by heart.
- The best way to learn these formulas is by doing lots of practice problems.
- Often, knowing the derivation of a formula will also help you remember it.
- Follow along with the lectures to fill in missing steps.


# Reflection identities

## Reflection across the $x$-axis (even/odd identities)

:::: {.columns }
::: {.column width="60%"}

Formulas:

\begin{empheq}[box=\fbox]{align*}
    \cos(-\theta) & = \phantom{-} \cos \theta \\
    \sin(-\theta) & = - \sin \theta
\end{empheq}

Example: Compute $\sin(-\pi/4)$

:::

::: {.column width="40%"}
![](./images/01-trigonometry/even-odd.svg)
:::
::::

## Reflection across the $y$-axis (complementary angles)

:::: {.columns }
::: {.column width="60%"}
Formulas:

\begin{empheq}[box=\fbox]{align*}
            \cos(\pi - \theta) & = - \cos\theta \\
            \sin(\pi - \theta) & = \phantom{-} \sin \theta
\end{empheq}

:::
::: {.column width="40%"}
![](./images/01-trigonometry/reflection-y.svg)
:::
::::

# Shift formulas

## Shift formulas (by $\pi$)

:::: {.columns }
::: {.column width="60%"}
Formulas:

\begin{empheq}[box=\fbox]{align*}
            \cos(\pi + \theta) & = - \cos \theta \\
            \sin(\pi + \theta) & = - \sin \theta \\
            \tan(\pi + \theta) & = \phantom{-} \tan\theta
\end{empheq}

:::
::: {.column width="40%"}
![](./images/01-trigonometry/shift-formulas.svg)
:::
::::

## Shift formulas (by $\pi/2$)

Formulas:

\begin{empheq}[box=\fbox]{align*}
            \sin \left( \frac{\pi}{2} - \theta\right) & = \cos \theta \\
            \cos \left( \frac{\pi}{2} - \theta\right) & = \sin \theta \\
            \tan \left( \frac{\pi}{2} - \theta\right) & = \cot \theta
\end{empheq}

- Proof skipped.
- **Very important formulas** to turn $\sin$ into $\cos$ and vice versa.

# Addition/subtraction formulas

## Addition/subtraction formulas (for $\sin$ and $\cos$)

Formulas:

\begin{empheq}[box=\fbox]{align*}
            \sin(\alpha + \beta) & = \sin \alpha \cos \beta + \cos \alpha \sin \beta \\
            \sin(\alpha - \beta) & = \sin \alpha \cos \beta - \cos \alpha \sin \beta \\
            \cos(\alpha + \beta) & = \cos \alpha \cos \beta - \sin \alpha \sin \beta \\
            \cos(\alpha - \beta) & = \cos \alpha \cos \beta + \sin \alpha \sin \beta
\end{empheq}

- Proof skipped.
- Note the signs for $\cos$!
- Every formula on the previous slides can be derived from these formulas.

## Example

Compute $\displaystyle \sin\left( \frac{7 \pi}{12} \right)$.

## Addition/subtraction formulas (for $\tan$)

Formulas:

\begin{empheq}[box=\fbox]{align*}
            \tan(\alpha + \beta) & = \frac{\tan \alpha + \tan \beta}{1 - \tan \alpha \tan \beta} \\
            \tan(\alpha - \beta) & = \frac{\tan \alpha - \tan \beta}{1 + \tan \alpha \tan \beta}
\end{empheq}

# Double/half angle formulas

## Double-angle formulas ($2\theta \to \theta$)

Formulas:

\begin{empheq}[box=\fbox]{align*}
            \sin(2 \theta) & = 2 \sin \theta \cos \theta \\
            \cos(2 \theta) & = \cos^2 \theta - \sin^2 \theta \\
            \tan(2 \theta) & = \frac{2 \tan \theta}{1 - \tan^2 \theta}
\end{empheq}

- Follows from the addition/subtraction formulas.
- The double-angle formula for $\cos$ can also be written as

\begin{empheq}[box=\fbox]{align*}
            \cos(2 \theta) & = \cos^2 \theta - \sin^2 \theta \\
                           & = 2 \cos^2 \theta - 1 \\
                           & = 1 - 2 \sin^2 \theta
\end{empheq}

## Example

Prove that $\displaystyle \tan\left(\frac{\pi}{4} + x\right) = \frac{1 + \tan x}{1 - \tan x}$.

## Half-angle formulas ($\theta \to 2\theta$)

Formulas:

\begin{empheq}[box=\fbox]{align*}
            \cos^2 \theta & = \frac{1 + \cos(2\theta)}{2} \\
            \sin^2 \theta & = \frac{1 - \cos(2\theta)}{2} \\            
            \tan^2 \theta & = \frac{1 - \cos(2\theta)}{1 + \cos(2\theta)}
\end{empheq}

These formulas are useful to compute integrals of powers of $\sin$ and $\cos$.

## Example

Express $\cos^2 x \sin^2 x$ as a combination of sines and cosines, without any powers.

# Formulas for product to sum and sum to product

## Product-to-sum formulas

Formulas:

\begin{empheq}[box=\fbox]{align*}
    \sin \alpha \cos \beta & = \frac{1}{2}(\sin(\alpha + \beta) + \sin(\alpha - \beta)) \\
    \cos \alpha \sin \beta & = \frac{1}{2}(\sin(\alpha + \beta) - \sin(\alpha - \beta)) \\
    \cos \alpha \cos \beta & = \frac{1}{2}(\cos(\alpha + \beta) + \cos(\alpha - \beta) \\
    \sin \alpha \sin \beta & = \frac{1}{2}(\cos(\alpha - \beta) - \cos(\alpha + \beta)
\end{empheq}


## Sum-to-product formulas

Formulas:

\begin{empheq}[box=\fbox]{align*}
            \sin \alpha + \sin \beta & = \phantom{-} 2\sin\left(\frac{\alpha+\beta}{2}\right) \cos\left(\frac{\alpha-\beta}{2}\right) \\
            \sin \alpha - \sin \beta & = \phantom{-} 2\cos\left(\frac{\alpha+\beta}{2}\right) \sin\left(\frac{\alpha-\beta}{2}\right) \\            
            \cos \alpha + \cos \beta & = \phantom{-} 2\cos\left(\frac{\alpha+\beta}{2}\right) \cos\left(\frac{\alpha-\beta}{2}\right) \\
            \cos \alpha - \cos \beta & = - 2\sin\left(\frac{\alpha+\beta}{2}\right) \sin\left(\frac{\alpha-\beta}{2}\right)
\end{empheq}

##

![](./images/01-trigonometry/hoodie-formulas.jpg){fig-align="center"}