---
title: "The binomial theorem"
subtitle: Introduction to Engineering Mathematics
author: Prof. Joris Vankerschaver
---


# Pascal's triangle

### Pascal's triangle

Expand the following expressions and look at the coefficients.

- $(a + b)^0 = 1$
- $(a + b)^1 = a + b$
- $(a + b)^2 = a^2 + 2ab + b^2$
- $(a + b)^3 = a^3 + 3a^2 b + 3ab^2 + b^3$
- $(a + b)^4 = a^4 + 4a^3 b + 6a^2 b^2 + 4ab^3 + b^4$
- $(a + b)^5 = a^5 + 5a^4b + 10a^3b^2 + 10a^2 b^3 + 5ab^4 + b^5$

What do you notice?

Based on this pattern, what is $(a + b)^7$?

Would you be able to write down $(a + b)^{27}$?

###

:::: {.columns }
::: {.column width="50%"}
![](./images/07-binomial/Yanghui_triangle.png){fig-align="center" height="500"}

[Jian Xian (贾宪), 11th century CE](https://en.wikipedia.org/wiki/Jia_Xian)

:::
::: {.column width="50%"}

![](./images/07-binomial/TrianguloPascal.jpeg){fig-align="center" height="500"}

[Blaise Pascal, 1665 CE](https://en.wikipedia.org/wiki/Pascal%27s_triangle)
:::
::::

Figures: Wikipedia.

### Example

Use Pascal's triangle to expand $\displaystyle \left(2x + \frac{1}{x}\right)^5$.

# Binomial coefficients

### Binomial coefficients

- Factorial: $n! = n(n-1)(n-2) \cdots 2 \cdot 1$.
- Binomial coefficient (also called "n-choose-k"):
$$
    {n \choose k} = C^k_n = \frac{n!}{k!(n-k)!}.
$$
- Measures the number of ways of choosing $k$ objects from among $n$ choices.

### Properties

For all $n$ and $k \le n$:

\begin{align*} 
    {n \choose 0} & = {n \choose n} = 1 \\
    {n \choose 1} & = {n \choose n - 1} = n \\
    {n \choose k} & = {n \choose n - k}
\end{align*}

### Rewriting Pascal's triangle using binomial coefficients

# The binomial theorem

### The binomial expansion

Putting everything we've learned together, we get
$$
    (a + b)^n = {n \choose 0} a^n b^0 + {n \choose 1} a^{n-1}b^1 + \cdots + {n \choose n-1} a^1 b^{n-1} + {n \choose n} a^0 b^n.
$$
This can be written more compactly as
$$
    (a + b)^n = \sum_{k = 0}^n {n \choose k} a^{n - k} b^k.
$$

### Example

Use the binomial expansion to expand $\displaystyle (\sqrt{x} - 1)^7$.

### Visual proof of the binomial expansion (optional)

![](./images/07-binomial/binomial-proof.png){fig-align="center"}
